wand_demo/bst_lemmas.v
@@ -21,16 +21,28 @@ Fixpoint tree_rep (t: tree val) (p: val) : mpred :=
 Definition treebox_rep (t: tree val) (b: val) :=
  EX p: val, data_at Tsh (tptr t_struct_tree) p b * tree_rep t p.
 
-(*
-(* TODO: seems not useful *)
+Lemma tree_rep_spec: forall (t: tree val) (p: val),
+  tree_rep t p =
+  match t with
+  | E => !!(p=nullval) && emp
+  | T a x v b => !! (Int.min_signed <= Z.of_nat x <= Int.max_signed /\ tc_val (tptr Tvoid) v) &&
+     EX pa:val, EX pb:val,
+     data_at Tsh t_struct_tree (Vint (Int.repr (Z.of_nat x)),(v,(pa,pb))) p *
+     tree_rep a pa * tree_rep b pb
+  end.
+Proof.
+  intros.
+  destruct t; auto.
+Qed.  
+
 Lemma treebox_rep_spec: forall (t: tree val) (b: val),
   treebox_rep t b =
-  EX p: val, 
+  EX p: val,
+  data_at Tsh (tptr t_struct_tree) p b *
   match t with
-  | E => !!(p=nullval) && data_at Tsh (tptr t_struct_tree) p b
-  | T l x v r => !! (Int.min_signed <= x <= Int.max_signed /\ tc_val (tptr Tvoid) v) &&
-      data_at Tsh (tptr t_struct_tree) p b *
-      field_at Tsh t_struct_tree [StructField _key] (Vint (Int.repr x)) p *
+  | E => !!(p=nullval) && emp
+  | T l x v r => !! (Int.min_signed <= Z.of_nat x <= Int.max_signed /\ tc_val (tptr Tvoid) v) &&
+      field_at Tsh t_struct_tree [StructField _key] (Vint (Int.repr (Z.of_nat x))) p *
       field_at Tsh t_struct_tree [StructField _value] v p *
       treebox_rep l (field_address t_struct_tree [StructField _left] p) *
       treebox_rep r (field_address t_struct_tree [StructField _right] p)
@@ -58,16 +70,51 @@ Proof.
       cancel.
 Qed.
 
+Lemma treebox_rep_tree_rep: forall (t: tree val) (b: val),
+  treebox_rep t b = EX p: val, data_at Tsh (tptr t_struct_tree) p b * tree_rep t p.
+Proof.
+  intros.
+  reflexivity.
+Qed.
 
-*)
+Lemma tree_rep_treebox_rep: forall (t: tree val) (p: val),
+  tree_rep t p =
+  match t with
+  | E => !!(p=nullval) && emp
+  | T l x v r => !! (Int.min_signed <= Z.of_nat x <= Int.max_signed /\ tc_val (tptr Tvoid) v) &&
+      field_at Tsh t_struct_tree [StructField _key] (Vint (Int.repr (Z.of_nat x))) p *
+      field_at Tsh t_struct_tree [StructField _value] v p *
+      treebox_rep l (field_address t_struct_tree [StructField _left] p) *
+      treebox_rep r (field_address t_struct_tree [StructField _right] p)
+  end.
+Proof.
+  intros.
+  destruct t; auto.
+  unfold treebox_rep; simpl.
+  apply pred_ext; Intros pa pb.
+  + Exists pb pa; entailer!.
+    unfold_data_at 1%nat.
+    cancel.
+    rewrite !field_at_data_at.
+    cancel.
+  + Exists pb pa; entailer!.
+    unfold_data_at 3%nat.
+    cancel.
+    rewrite !field_at_data_at.
+    cancel.
+Qed.
 
+Arguments tree_rep: simpl never.
+Arguments treebox_rep: simpl never.
+Opaque treebox_rep tree_rep.
 
 Lemma tree_rep_saturate_local:
    forall t p, tree_rep t p |-- !! is_pointer_or_null p.
 Proof.
-destruct t; simpl; intros.
-entailer!.
-Intros pa pb. entailer!.
+  intros.
+  rewrite tree_rep_treebox_rep.
+  destruct t;
+  entailer!.
 Qed.
 
 Hint Resolve tree_rep_saturate_local: saturate_local.
@@ -75,8 +122,14 @@ Hint Resolve tree_rep_saturate_local: saturate_local.
 Lemma tree_rep_valid_pointer:
   forall t p, tree_rep t p |-- valid_pointer p.
 Proof.
-intros.
-destruct t; simpl; normalize; auto with valid_pointer.
+  intros.
+  rewrite tree_rep_treebox_rep.
+  destruct t; simpl;
+   normalize;
+   auto with valid_pointer.
+  repeat apply sepcon_valid_pointer1.
+  apply field_at_valid_ptr0; auto.
+  reflexivity.
 Qed.
 Hint Resolve tree_rep_valid_pointer: valid_pointer.
 
@@ -84,8 +137,9 @@ Lemma treebox_rep_saturate_local:
    forall t b, treebox_rep t b |-- !! field_compatible (tptr t_struct_tree) [] b.
 Proof.
 intros.
-unfold treebox_rep.
+rewrite treebox_rep_spec.
 Intros p.
+destruct t;
 entailer!.
 Qed.
 
@@ -96,8 +150,8 @@ Lemma tree_rep_nullval: forall t,
 Proof.
   intros.
   destruct t; [entailer! |].
-  simpl tree_rep.
-  Intros pa pb. entailer!.
+  rewrite tree_rep_treebox_rep.
+  entailer!.
 Qed.
 
 Hint Resolve tree_rep_nullval: saturate_local.
@@ -108,74 +162,74 @@ Lemma treebox_rep_leaf: forall x p b (v: val),
   data_at Tsh t_struct_tree (Vint (Int.repr (Z.of_nat x)), (v, (nullval, nullval))) p * data_at Tsh (tptr t_struct_tree) p b |-- treebox_rep (T E x v E) b.
 Proof.
   intros.
-  unfold treebox_rep, tree_rep. Exists p nullval nullval. entailer!.
+  rewrite treebox_rep_spec.
+  Exists p.
+  rewrite !treebox_rep_spec.
+  Exists nullval nullval.
+  unfold_data_at 1%nat.
+  entailer!.
+  rewrite !field_at_data_at.
+  cancel.
 Qed.
 
 Module PartialTreeboxRep_WandFrame.
 
-Lemma partial_treebox_rep_singleton_left: forall (t1 t1' t2: tree val) k (v p1 p2 p b: val),
+Lemma partial_treebox_rep_singleton_left: forall (t1' t2: tree val) k (v p b: val),
   Int.min_signed <= Z.of_nat k <= Int.max_signed ->
   is_pointer_or_null v ->
   data_at Tsh (tptr t_struct_tree) p b *
-  data_at Tsh t_struct_tree (Vint (Int.repr (Z.of_nat k)), (v, (p1, p2))) p *
-  tree_rep t1 p1 * tree_rep t2 p2
-  |-- treebox_rep t1 (field_address t_struct_tree [StructField _left] p) *
-       (treebox_rep t1'
-         (field_address t_struct_tree [StructField _left] p) -*
-        treebox_rep (T t1' k v t2) b).
+  field_at Tsh t_struct_tree [StructField _key] (Vint (Int.repr (Z.of_nat k))) p *
+  field_at Tsh t_struct_tree [StructField _value] v p *
+  treebox_rep t2 (field_address t_struct_tree [StructField _right] p)
+  |-- treebox_rep t1'
+        (field_address t_struct_tree [StructField _left] p) -*
+      treebox_rep (T t1' k v t2) b.
 Proof.
   intros.
-  unfold_data_at 2%nat.
-  rewrite (field_at_data_at _ t_struct_tree [StructField _left]).
-  unfold treebox_rep at 1. Exists p1. cancel.
-
+  rewrite (treebox_rep_spec (T t1' k v t2)).
   rewrite <- wand_sepcon_adjoint.
-  clear p1.
-  unfold treebox_rep.
   Exists p.
-  simpl.
-  Intros p1.
-  Exists p1 p2.
   entailer!.
-  unfold_data_at 2%nat.
-  rewrite (field_at_data_at _ t_struct_tree [StructField _left]).
-  cancel.
 Qed.
 
-Lemma partial_treebox_rep_singleton_right: forall (t1 t2 t2': tree val) k (v p1 p2 p b: val),
+Lemma partial_treebox_rep_singleton_right: forall (t1 t2': tree val) k (v p b: val),
   Int.min_signed <= Z.of_nat k <= Int.max_signed ->
   is_pointer_or_null v ->
   data_at Tsh (tptr t_struct_tree) p b *
-  data_at Tsh t_struct_tree (Vint (Int.repr (Z.of_nat k)), (v, (p1, p2))) p *
-  tree_rep t1 p1 * tree_rep t2 p2
-  |-- treebox_rep t2 (field_address t_struct_tree [StructField _right] p) *
-       (treebox_rep t2'
-         (field_address t_struct_tree [StructField _right] p) -*
-        treebox_rep (T t1 k v t2') b).
+  field_at Tsh t_struct_tree [StructField _key] (Vint (Int.repr (Z.of_nat k))) p *
+  field_at Tsh t_struct_tree [StructField _value] v p *
+  treebox_rep t1 (field_address t_struct_tree [StructField _left] p)
+  |-- treebox_rep t2'
+       (field_address t_struct_tree [StructField _right] p) -*
+      treebox_rep (T t1 k v t2') b.
 Proof.
   intros.
-  unfold_data_at 2%nat.
-  rewrite (field_at_data_at _ t_struct_tree [StructField _right]).
-  unfold treebox_rep at 1. Exists p2. cancel.
-
+  rewrite (treebox_rep_spec (T t1 k v t2')).
   rewrite <- wand_sepcon_adjoint.
-  clear p2.
-  unfold treebox_rep.
   Exists p.
-  simpl.
-  Intros p2.
-  Exists p1 p2.
   entailer!.
-  unfold_data_at 2%nat.
-  rewrite (field_at_data_at _ t_struct_tree [StructField _right]).
-  cancel.
 Qed.
 
-Lemma partial_treebox_rep_partial_tree_rep: forall t1 t2 t3 p1 p2 p3,
+Lemma partial_treebox_rep_partial_treebox_rep: forall t1 t2 t3 p1 p2 p3,
   (treebox_rep t1 p1 -* treebox_rep t2 p2) * (treebox_rep t2 p2 -* treebox_rep t3 p3) |-- treebox_rep t1 p1 -* treebox_rep t3 p3.
 Proof.
   intros.
   apply wand_frame_ver.
+Qed.
+
+Lemma emp_partial_treebox_rep_H: forall t p,
+  emp |-- treebox_rep t p -* treebox_rep t p.
+Proof.
+  intros.
+  apply wand_sepcon_adjoint.
+  normalize.
+Qed.
+
+Lemma treebox_rep_partial_treebox_rep: forall t t0 p p0,
+  treebox_rep t p * (treebox_rep t p -* treebox_rep t0 p0) |-- treebox_rep t0 p0.
+Proof.
+  intros.
+  apply modus_ponens_wand.
 Qed.
 
 End PartialTreeboxRep_WandFrame.
@@ -185,63 +239,72 @@ Module PartialTreeboxRep_WandQFrame.
 Definition partial_treebox_rep (pt: partial_tree val) (p_root p_in: val): mpred :=
   ALL t: tree val, treebox_rep t p_in -* treebox_rep (partial_tree_tree pt t) p_root.
 
-Lemma partial_treebox_rep_singleton_left: forall (t1 t1' t2: tree val) k (v p1 p2 p b: val),
+Lemma partial_treebox_rep_singleton_left: forall (t2: tree val) k (v p b: val),
   Int.min_signed <= Z.of_nat k <= Int.max_signed ->
   is_pointer_or_null v ->
   data_at Tsh (tptr t_struct_tree) p b *
-  data_at Tsh t_struct_tree (Vint (Int.repr (Z.of_nat k)), (v, (p1, p2))) p *
-  tree_rep t1 p1 * tree_rep t2 p2
-  |-- treebox_rep t1 (field_address t_struct_tree [StructField _left] p) *
-       (treebox_rep t1'
-         (field_address t_struct_tree [StructField _left] p) -*
-        treebox_rep (T t1' k v t2) b).
+  field_at Tsh t_struct_tree [StructField _key] (Vint (Int.repr (Z.of_nat k))) p *
+  field_at Tsh t_struct_tree [StructField _value] v p *
+  treebox_rep t2 (field_address t_struct_tree [StructField _right] p)
+  |-- partial_treebox_rep (L H k v t2) b (field_address t_struct_tree [StructField _left] p).
 Proof.
   intros.
-  unfold_data_at 2%nat.
-  rewrite (field_at_data_at _ t_struct_tree [StructField _left]).
-  unfold treebox_rep at 1. Exists p1. cancel.
-
+  unfold partial_treebox_rep.
+  apply allp_right; intros t1.
   rewrite <- wand_sepcon_adjoint.
-  clear p1.
-  unfold treebox_rep.
+  rewrite (treebox_rep_spec (T t1 k v t2)).
   Exists p.
-  simpl.
-  Intros p1.
-  Exists p1 p2.
   entailer!.
-  unfold_data_at 2%nat.
-  rewrite (field_at_data_at _ t_struct_tree [StructField _left]).
-  cancel.
 Qed.
 
-Lemma partial_treebox_rep_singleton_right: forall (t1 t2 t2': tree val) k (v p1 p2 p b: val),
+Lemma partial_treebox_rep_singleton_right: forall (t1: tree val) k (v p b: val),
   Int.min_signed <= Z.of_nat k <= Int.max_signed ->
   is_pointer_or_null v ->
   data_at Tsh (tptr t_struct_tree) p b *
-  data_at Tsh t_struct_tree (Vint (Int.repr (Z.of_nat k)), (v, (p1, p2))) p *
-  tree_rep t1 p1 * tree_rep t2 p2
-  |-- treebox_rep t2 (field_address t_struct_tree [StructField _right] p) *
-       (treebox_rep t2'
-         (field_address t_struct_tree [StructField _right] p) -*
-        treebox_rep (T t1 k v t2') b).
+  field_at Tsh t_struct_tree [StructField _key] (Vint (Int.repr (Z.of_nat k))) p *
+  field_at Tsh t_struct_tree [StructField _value] v p *
+  treebox_rep t1 (field_address t_struct_tree [StructField _left] p)
+  |-- partial_treebox_rep (R t1 k v H) b (field_address t_struct_tree [StructField _right] p).
 Proof.
   intros.
-  unfold_data_at 2%nat.
-  rewrite (field_at_data_at _ t_struct_tree [StructField _right]).
-  unfold treebox_rep at 1. Exists p2. cancel.
-
+  unfold partial_treebox_rep.
+  apply allp_right; intros t2.
   rewrite <- wand_sepcon_adjoint.
-  clear p2.
-  unfold treebox_rep.
+  rewrite (treebox_rep_spec (T t1 k v t2)).
   Exists p.
-  simpl.
-  Intros p2.
-  Exists p1 p2.
   entailer!.
-  unfold_data_at 2%nat.
-  rewrite (field_at_data_at _ t_struct_tree [StructField _right]).
-  cancel.
 Qed.
 
-Lemma partial_treebox_rep_partial_tree_rep: forall t1 t2 t3 p1 p2 p3,
-  (treebox_rep t1 p1 -* treebox_rep t2 p2) * (treebox_rep t2 p2 -* treebox_rep t3 p3) |-- treebox_rep t1 p1 -* treebox_rep t3 p3.
+Lemma partial_treebox_rep_partial_treebox_rep: forall pt12 pt23 p1 p2 p3,
+  partial_treebox_rep pt12 p2 p1 * partial_treebox_rep pt23 p3 p2 |-- partial_treebox_rep (partial_tree_partial_tree pt23 pt12) p3 p1.
+Proof.
+  intros.
+  unfold partial_treebox_rep.
+  rewrite partial_tree_partial_tree_tree.
+  sep_apply (wandQ_frame_refine _ _ (fun t => treebox_rep t p2 -* treebox_rep (partial_tree_tree pt23 t) p3) (partial_tree_tree pt12)).
+  rewrite sepcon_comm.
+  apply wandQ_frame_ver.
+Qed.
+
+Lemma emp_partial_treebox_rep_H: forall p,
+  emp |-- partial_treebox_rep SearchTree_ext.H p p.
+Proof.
+  intros.
+  apply allp_right; intros.
+  apply wand_sepcon_adjoint.
+  normalize.
+Qed.
+
+Lemma treebox_rep_partial_treebox_rep: forall t pt p q,
+  treebox_rep t p * partial_treebox_rep pt q p |-- treebox_rep (partial_tree_tree pt t) q.
+Proof.
+  intros.
+  unfold partial_treebox_rep.
+  change (treebox_rep (partial_tree_tree pt t) q)
+    with ((fun t => treebox_rep (partial_tree_tree pt t) q) t).
+  change (treebox_rep t p)
+    with ((fun t => treebox_rep t p) t).
+  apply wandQ_frame_elim.
+Qed.
+
+End PartialTreeboxRep_WandQFrame.
